ComposableModules.v
@@ -14,43 +14,43 @@ Inductive ModuleType : Type :=
 
 Fixpoint ModuleSem (mt : ModuleType) (t_acc : Tree Elem) (t_curr : Tree Elem) : Type :=
   match mt with
-  | MkMod => Mod (Node "" [t_acc; t_curr])
+  | MkMod => Mod t_acc
   | MkMeth K_in K_out => type K_in -> Action type t_curr K_out
-  | BindMod B => forall (t_new : Tree Elem), Mod t_new -> ModuleSem B (Node "" [t_acc; t_curr]) t_new
+  | BindMod B => forall (t_new : Tree Elem), Mod t_new -> ModuleSem B (Node "" [t_acc; t_new]) t_new
   | BindMeth K_in K_out B => (type K_in -> Action type t_curr K_out) -> ModuleSem B t_acc t_curr
   end.
 
-Definition MethInclusion {t1 t2: Tree Elem} {K_in K_out: Kind}
+Definition MethSimulation {t1 t2: Tree Elem} {K_in K_out: Kind}
   (M1: type K_in -> Action type t1 K_out) (M2: type K_in -> Action type t2 K_out)
   (rel: TreeState ElemState t1 -> TreeState ElemState t2 -> Prop) : Prop :=
   forall (v_in : type K_in),
-    ActionInclusion (M1 v_in) (M2 v_in) rel.
+    ActionSimulation (M1 v_in) (M2 v_in) rel.
 
-Fixpoint Rel (mt : ModuleType)
-             (t_acc1 t_acc2 : Tree Elem)
-             (rel_acc : TreeState ElemState t_acc1 -> TreeState ElemState t_acc2 -> Prop)
-             (t_curr1 t_curr2 : Tree Elem)
-             (rel_curr : TreeState ElemState t_curr1 -> TreeState ElemState t_curr2 -> Prop)
-             (m1 : ModuleSem mt t_acc1 t_curr1) (m2 : ModuleSem mt t_acc2 t_curr2) : Prop :=
+Fixpoint Simulation (mt : ModuleType)
+                     (t_acc1 t_acc2 : Tree Elem)
+                     (rel_acc : TreeState ElemState t_acc1 -> TreeState ElemState t_acc2 -> Prop)
+                     (t_curr1 t_curr2 : Tree Elem)
+                     (rel_curr : TreeState ElemState t_curr1 -> TreeState ElemState t_curr2 -> Prop)
+                     (m1 : ModuleSem mt t_acc1 t_curr1) (m2 : ModuleSem mt t_acc2 t_curr2) : Prop :=
   match mt as mt0 return ModuleSem mt0 t_acc1 t_curr1 -> ModuleSem mt0 t_acc2 t_curr2 -> Prop with
   | MkMod => fun m1 m2 =>
-      ModInclusion m1 m2 (fun s1 s2 => rel_acc s1.(Fst) s2.(Fst) /\ rel_curr s1.(Snd).(Fst) s2.(Snd).(Fst))
+      ModSimulation m1 m2 rel_acc
   | MkMeth K_in K_out => fun m1 m2 =>
-      MethInclusion m1 m2 rel_curr
+      MethSimulation m1 m2 rel_curr
   | BindMod B => fun F1 F2 =>
       forall (t_new1 t_new2 : Tree Elem)
              (m1_in : Mod t_new1)
              (m2_in : Mod t_new2)
              (rel_new : TreeState ElemState t_new1 -> TreeState ElemState t_new2 -> Prop),
-        ModInclusion m1_in m2_in rel_new ->
-        Rel B (Node "" [t_acc1; t_curr1]) (Node "" [t_acc2; t_curr2])
-            (fun s1 s2 => rel_acc s1.(Fst) s2.(Fst) /\ rel_curr s1.(Snd).(Fst) s2.(Snd).(Fst))
+        ModSimulation m1_in m2_in rel_new ->
+        Simulation B (Node "" [t_acc1; t_new1]) (Node "" [t_acc2; t_new2])
+            (fun s1 s2 => rel_acc s1.(Fst) s2.(Fst) /\ rel_new s1.(Snd).(Fst) s2.(Snd).(Fst))
             t_new1 t_new2
             rel_new
             (F1 t_new1 m1_in)
             (F2 t_new2 m2_in)
   | BindMeth K_in K_out B => fun F1 F2 =>
       forall (M1 : type K_in -> Action type t_curr1 K_out) (M2 : type K_in -> Action type t_curr2 K_out),
-        MethInclusion M1 M2 rel_curr ->
-        Rel B t_acc1 t_acc2 rel_acc t_curr1 t_curr2 rel_curr (F1 M1) (F2 M2)
+        MethSimulation M1 M2 rel_curr ->
+        Simulation B t_acc1 t_acc2 rel_acc t_curr1 t_curr2 rel_curr (F1 M1) (F2 M2)
   end m1 m2.
